Model nontermination explicitly ("partial Hurd monad") (#104)
This PR changes the type of `Monad.Result<A>` from `Result(value: A,
rest: Rand.Bitstream)` to `Diverging | Result(value: A, rest:
Rand.Bitstream)`. In order to make it easier to work with, it also adds
a few combinators for `Monad.Result` in order to avoid pattern matching
everywhere.

The main benefit of this is that `While` loops can be properly defined
without `assume false` and we can prove Hurd's theorem 38 (while loop
unrolling) in Dafny. Another benefit is that we can reason about
nontermination probabilities in Dafny via `Rand.prob(iset s |
Sample(s).Diverging?)` for a probabilistic computation `Sample:
Hurd<A>`.

For reasoning about the measurability of results, I also introduced some
infrastructure to lift measure spaces on `A` to `Result<A>`, see
`Monad.ResultEventSpace`, `Monad.LiftInEventSpaceToResultEventSpace`,
and `Monad.LiftRestInEventSpaceToResultEventSpace`. In fact, the
measurability proofs required the most modifications as a result of the
change.

By submitting this pull request, I confirm that my contribution is made
under the terms of the [MIT
license](https://github.com/dafny-lang/dafny/blob/master/LICENSE.txt).

src/Distributions/UniformPowerOfTwo/Correctness.dfy
@@ -23,7 +23,7 @@ module UniformPowerOfTwo.Correctness {
     Rand.prob(iset s | Model.Sample(n)(s).value == m) == if m < Helper.Power(2, k) then 1.0 / (Helper.Power(2, k) as real) else 0.0
   }
 
-  function Sample1(n: nat): Rand.Bitstream -> Rand.Bitstream
+  function SampleRest(n: nat): Rand.Bitstream -> Rand.Bitstream
     requires n >= 1
   {
     (s: Rand.Bitstream) => Model.Sample(n)(s).rest
@@ -47,13 +47,14 @@ module UniformPowerOfTwo.Correctness {
     var k := Helper.Log2Floor(n);
 
     assert e in Rand.eventSpace by {
-      assert iset{m} in Measures.natEventSpace;
-      var preimage := Measures.PreImage((s: Rand.Bitstream) => Model.Sample(n)(s).value, iset{m});
-      assert preimage in Rand.eventSpace by {
-        assert Measures.IsMeasurable(Rand.eventSpace, Measures.natEventSpace, s => Model.Sample(n)(s).value) by {
-          SampleIsIndep(n);
-          Independence.IsIndepImpliesValueMeasurableNat(Model.Sample(n));
-        }
+      var resultsWithValueM := Monad.ResultsWithValueIn(iset{m});
+      assert resultsWithValueM in Monad.natResultEventSpace by {
+        Monad.LiftInEventSpaceToResultEventSpace(iset{m}, Measures.natEventSpace);
+      }
+      var preimage := Measures.PreImage(Model.Sample(n), resultsWithValueM);
+      assert Measures.IsMeasurable(Rand.eventSpace, Monad.natResultEventSpace, Model.Sample(n)) by {
+        SampleIsIndep(n);
+        Independence.IsIndepImpliesMeasurableNat(Model.Sample(n));
       }
       assert e == preimage;
     }
@@ -184,13 +185,22 @@ module UniformPowerOfTwo.Correctness {
 
   lemma SampleIsMeasurePreserving(n: nat)
     requires n >= 1
-    ensures Measures.IsMeasurePreserving(Rand.eventSpace, Rand.prob, Rand.eventSpace, Rand.prob, Sample1(n))
+    ensures Measures.IsMeasurePreserving(Rand.eventSpace, Rand.prob, Rand.eventSpace, Rand.prob, SampleRest(n))
   {
-    var f := Sample1(n);
+    var f := SampleRest(n);
     assert Measures.IsMeasurable(Rand.eventSpace, Rand.eventSpace, f) by {
-      SampleIsIndep(n);
-      Independence.IsIndepImpliesRestMeasurable(Model.Sample(n));
-      assert Independence.IsIndep(Model.Sample(n));
+      forall e | e in Rand.eventSpace ensures Measures.PreImage(f, e) in Rand.eventSpace {
+        var resultsWithRestInE := Monad.ResultsWithRestIn(e);
+        assert resultsWithRestInE in Monad.natResultEventSpace by {
+          Monad.LiftRestInEventSpaceToResultEventSpace(e, Measures.natEventSpace);
+        }
+        var preimage' := Measures.PreImage(Model.Sample(n), resultsWithRestInE);
+        assert preimage' in Rand.eventSpace by {
+          SampleIsIndep(n);
+          Independence.IsIndepImpliesMeasurableNat(Model.Sample(n));
+        }
+        assert Measures.PreImage(f, e) == preimage';
+      }
     }
     if n == 1 {
       forall e | e in Rand.eventSpace ensures Rand.prob(Measures.PreImage(f, e)) == Rand.prob(e) {
@@ -202,7 +212,7 @@ module UniformPowerOfTwo.Correctness {
       }
       assert Measures.IsMeasurePreserving(Rand.eventSpace, Rand.prob, Rand.eventSpace, Rand.prob, f);
     } else {
-      var g := Sample1(n / 2);
+      var g := SampleRest(n / 2);
       forall e | e in Rand.eventSpace ensures Rand.prob(Measures.PreImage(f, e)) == Rand.prob(e) {
         var e' := (iset s | Rand.Tail(s) in e);
         assert e' in Rand.eventSpace by {
@@ -309,8 +319,8 @@ module UniformPowerOfTwo.Correctness {
     var E: iset<Rand.Bitstream> := (iset s | m % 2 as nat == Helper.boolToNat(Monad.Coin(s).value));
     var f := (s: Rand.Bitstream) => Model.Sample(n / 2)(s).rest;
 
-    var e1 := (iset s | Model.Sample(n / 2)(s).rest in E);
-    var e2 := (iset s | Model.Sample(n / 2)(s).value in A);
+    var e1 := (iset s | Model.Sample(n / 2)(s).RestIn(E));
+    var e2 := (iset s | Model.Sample(n / 2)(s).In(A));
     var e3 := (iset s | 2*aOf(s) + Helper.boolToNat(bOf(s)) == m);
 
     assert SplitEvent: e3 == e1 * e2 by {
